.lake/build/ir/IVI/Invariant.c
@@ -13,27 +13,22 @@
 #ifdef __cplusplus
 extern "C" {
 #endif
+static lean_object* l_IVI_reprNonCollapseCfg___redArg___closed__4____x40_IVI_Invariant___hyg_1654_;
 lean_object* l_Float_repr(double, lean_object*);
 LEAN_EXPORT lean_object* l_IVI_invariantProps___boxed(lean_object*, lean_object*, lean_object*, lean_object*, lean_object*, lean_object*);
-static lean_object* l_IVI_reprNonCollapseCfg___redArg___closed__9____x40_IVI_Invariant___hyg_1716_;
 lean_object* l_List_lengthTR___redArg(lean_object*);
 LEAN_EXPORT lean_object* l_IVI_Invariant_runUntilConverged_loop___boxed(lean_object*, lean_object*, lean_object*, lean_object*, lean_object*, lean_object*, lean_object*, lean_object*, lean_object*, lean_object*);
 double lean_float_mul(double, double);
-static lean_object* l_IVI_reprNonCollapseCfg___redArg___closed__6____x40_IVI_Invariant___hyg_1716_;
 LEAN_EXPORT lean_object* l_List_foldl___at___IVI_Invariant_resonanceMatrixW_spec__1___boxed(lean_object*, lean_object*);
 LEAN_EXPORT lean_object* l___private_IVI_Invariant_0__IVI_Invariant_vectorMaxDiff_match__1_splitter___redArg(lean_object*, lean_object*, lean_object*, lean_object*, lean_object*, lean_object*);
 LEAN_EXPORT lean_object* l_IVI_Invariant_spectralInvariantW___boxed(lean_object*, lean_object*);
 LEAN_EXPORT lean_object* l_List_mapTR_loop___at___IVI_Invariant_mulMatVec_spec__1(lean_object*, lean_object*, lean_object*);
 LEAN_EXPORT lean_object* l_IVI_zipIdx___redArg(lean_object*);
-static lean_object* l_IVI_reprNonCollapseCfg___redArg___closed__14____x40_IVI_Invariant___hyg_1716_;
-static lean_object* l_IVI_reprNonCollapseCfg___redArg___closed__4____x40_IVI_Invariant___hyg_1716_;
 LEAN_EXPORT lean_object* l_List_mapTR_loop___at___IVI_Invariant_resonanceMatrixW_spec__0(lean_object*, lean_object*, lean_object*, lean_object*, lean_object*);
 LEAN_EXPORT lean_object* l_IVI_Invariant_defaultWeighting___lam__0___boxed(lean_object*, lean_object*);
-static lean_object* l_IVI_reprNonCollapseCfg___redArg___closed__15____x40_IVI_Invariant___hyg_1716_;
 LEAN_EXPORT lean_object* l_IVI_Invariant_powerIter(lean_object*, lean_object*, double);
-static lean_object* l_IVI_reprNonCollapseCfg___redArg___closed__16____x40_IVI_Invariant___hyg_1716_;
 double lean_float_div(double, double);
-LEAN_EXPORT lean_object* l_IVI_reprNonCollapseCfg___redArg____x40_IVI_Invariant___hyg_1716_(lean_object*);
+static lean_object* l_IVI_reprNonCollapseCfg___redArg___closed__7____x40_IVI_Invariant___hyg_1654_;
 LEAN_EXPORT lean_object* l___private_IVI_Invariant_0__IVI_Invariant_normInf_match__1_splitter___boxed(lean_object*, lean_object*, lean_object*, lean_object*);
 LEAN_EXPORT lean_object* l___private_IVI_Invariant_0__IVI_Invariant_powerIterAux_match__1_splitter___redArg___boxed(lean_object*, lean_object*, lean_object*, lean_object*, lean_object*);
 LEAN_EXPORT double l_IVI_Invariant_spectralInvariant(lean_object*);
@@ -41,15 +36,13 @@ LEAN_EXPORT lean_object* l_List_foldrTR___at___IVI_Invariant_coarse_spec__0(lean
 LEAN_EXPORT double l_IVI_Invariant_fmax(double, double);
 LEAN_EXPORT lean_object* l___private_IVI_Invariant_0__IVI_Invariant_vectorMaxDiff_match__1_splitter___boxed(lean_object*, lean_object*, lean_object*, lean_object*, lean_object*, lean_object*, lean_object*);
 uint8_t lean_usize_dec_eq(size_t, size_t);
-static lean_object* l_IVI_reprNonCollapseCfg___redArg___closed__12____x40_IVI_Invariant___hyg_1716_;
 LEAN_EXPORT lean_object* l___private_IVI_Invariant_0__IVI_Invariant_vectorMaxDiff_match__1_splitter(lean_object*, lean_object*, lean_object*, lean_object*, lean_object*, lean_object*, lean_object*);
-LEAN_EXPORT lean_object* l_IVI_reprNonCollapseCfg____x40_IVI_Invariant___hyg_1716____boxed(lean_object*, lean_object*);
 LEAN_EXPORT lean_object* l_List_foldl___at___IVI_Invariant_mulMatVec_spec__0___boxed(lean_object*, lean_object*);
 double l_IVI_align(double, double);
 LEAN_EXPORT lean_object* l_IVI_Invariant_coarse(lean_object*);
 uint8_t lean_float_decLt(double, double);
 LEAN_EXPORT double l_List_foldl___at___IVI_Invariant_resonanceMatrixW_spec__1(double, lean_object*);
-static lean_object* l_IVI_reprNonCollapseCfg___redArg___closed__7____x40_IVI_Invariant___hyg_1716_;
+static lean_object* l_IVI_reprNonCollapseCfg___redArg___closed__0____x40_IVI_Invariant___hyg_1654_;
 LEAN_EXPORT lean_object* l___private_IVI_Invariant_0__IVI_Invariant_normInf_match__1_splitter___redArg___boxed(lean_object*, lean_object*, lean_object*);
 LEAN_EXPORT lean_object* l___private_IVI_Invariant_0__IVI_Invariant_normInf_match__1_splitter___redArg(lean_object*, lean_object*, lean_object*);
 LEAN_EXPORT double l_List_foldl___at___IVI_rowEntropy_spec__1(lean_object*, double, lean_object*);
@@ -73,29 +66,29 @@ LEAN_EXPORT lean_object* l_IVI_listGetD___redArg___boxed(lean_object*, lean_obje
 lean_object* lean_nat_to_int(lean_object*);
 LEAN_EXPORT lean_object* l___private_IVI_Invariant_0__IVI_Invariant_normInf_match__1_splitter(lean_object*, lean_object*, lean_object*, lean_object*);
 static double l_IVI_favg___closed__0;
+static lean_object* l_IVI_reprNonCollapseCfg___redArg___closed__9____x40_IVI_Invariant___hyg_1654_;
+LEAN_EXPORT lean_object* l_IVI_reprNonCollapseCfg___redArg____x40_IVI_Invariant___hyg_1654_(lean_object*);
 LEAN_EXPORT lean_object* l_IVI_Invariant_defaultWeighting;
-static lean_object* l_IVI_reprNonCollapseCfg___redArg___closed__0____x40_IVI_Invariant___hyg_1716_;
 lean_object* l_List_range(lean_object*);
 LEAN_EXPORT lean_object* l_IVI_rowEntropy___boxed(lean_object*);
 LEAN_EXPORT double l_List_foldl___at___List_foldl___at___IVI_rowEntropy_spec__1_spec__1(lean_object*, double, lean_object*);
 LEAN_EXPORT lean_object* l___private_IVI_Invariant_0__IVI_Invariant_powerIterAux_match__1_splitter(lean_object*, lean_object*, double, lean_object*, lean_object*, lean_object*);
-LEAN_EXPORT lean_object* l_IVI_reprNonCollapseCfg____x40_IVI_Invariant___hyg_1716_(lean_object*, lean_object*);
 double lean_float_of_nat(lean_object*);
 double log(double);
 LEAN_EXPORT lean_object* l_IVI_Invariant_vectorMaxDiff___boxed(lean_object*, lean_object*);
+LEAN_EXPORT lean_object* l_IVI_reprNonCollapseCfg____x40_IVI_Invariant___hyg_1654____boxed(lean_object*, lean_object*);
 LEAN_EXPORT lean_object* l___private_IVI_Invariant_0__IVI_Invariant_lambdaVector_match__1_splitter___redArg___boxed(lean_object*, lean_object*, lean_object*, lean_object*, lean_object*, lean_object*);
-static lean_object* l_IVI_reprNonCollapseCfg___redArg___closed__10____x40_IVI_Invariant___hyg_1716_;
 lean_object* l_List_replicateTR___redArg(lean_object*, lean_object*);
 static lean_object* l_IVI_instReprNonCollapseCfg___closed__0;
 LEAN_EXPORT lean_object* l_IVI_Invariant_enumerate(lean_object*, lean_object*);
 LEAN_EXPORT lean_object* l___private_IVI_Invariant_0__IVI_Invariant_lambdaVector_match__1_splitter___boxed(lean_object*, lean_object*, lean_object*, lean_object*, lean_object*, lean_object*, lean_object*);
+static lean_object* l_IVI_reprNonCollapseCfg___redArg___closed__3____x40_IVI_Invariant___hyg_1654_;
 LEAN_EXPORT double l_List_foldl___at___IVI_rowEntropy_spec__0(double, double, double, lean_object*);
 LEAN_EXPORT lean_object* l_IVI_listGetD___redArg(lean_object*, lean_object*, lean_object*);
 LEAN_EXPORT lean_object* l_IVI_Invariant_clampZero___boxed(lean_object*);
-static lean_object* l_IVI_reprNonCollapseCfg___redArg___closed__11____x40_IVI_Invariant___hyg_1716_;
 LEAN_EXPORT lean_object* l_IVI_Invariant_fmax___boxed(lean_object*, lean_object*);
-static lean_object* l_IVI_reprNonCollapseCfg___redArg___closed__5____x40_IVI_Invariant___hyg_1716_;
-static lean_object* l_IVI_reprNonCollapseCfg___redArg___closed__8____x40_IVI_Invariant___hyg_1716_;
+static lean_object* l_IVI_reprNonCollapseCfg___redArg___closed__1____x40_IVI_Invariant___hyg_1654_;
+static lean_object* l_IVI_reprNonCollapseCfg___redArg___closed__6____x40_IVI_Invariant___hyg_1654_;
 LEAN_EXPORT uint8_t l_IVI_surpriseNonDecreasing(lean_object*, lean_object*);
 LEAN_EXPORT lean_object* l_List_mapTR_loop___at___IVI_symmetriseLL_spec__0___boxed(lean_object*, lean_object*, lean_object*, lean_object*);
 static double l_IVI_Invariant_spectralInvariantW___closed__0;
@@ -106,26 +99,28 @@ LEAN_EXPORT lean_object* l_IVI_invariantProps(lean_object*, double, double, lean
 LEAN_EXPORT lean_object* l_IVI_instReprNonCollapseCfg;
 LEAN_EXPORT lean_object* l_List_mapTR_loop___at___IVI_Invariant_resonanceMatrixW_spec__2___boxed(lean_object*, lean_object*, lean_object*);
 double l_Float_ofScientific(lean_object*, uint8_t, lean_object*);
+static lean_object* l_IVI_reprNonCollapseCfg___redArg___closed__5____x40_IVI_Invariant___hyg_1654_;
 LEAN_EXPORT double l_IVI_Invariant_vectorMaxDiff(lean_object*, lean_object*);
 static double l_IVI_Invariant_powerIter___closed__0;
 LEAN_EXPORT lean_object* l_IVI_Invariant_lambdaVector(lean_object*, lean_object*, lean_object*);
 LEAN_EXPORT lean_object* l_List_mapTR_loop___at___IVI_symmetriseLL_spec__1___boxed(lean_object*, lean_object*, lean_object*);
 LEAN_EXPORT lean_object* l_IVI_Invariant_normInf___boxed(lean_object*);
 LEAN_EXPORT lean_object* l_IVI_Invariant_powerIter___boxed(lean_object*, lean_object*, lean_object*);
+static lean_object* l_IVI_reprNonCollapseCfg___redArg___closed__15____x40_IVI_Invariant___hyg_1654_;
 LEAN_EXPORT lean_object* l_List_mapTR_loop___at___List_mapTR_loop___at___IVI_symmetriseLL_spec__1_spec__1___boxed(lean_object*, lean_object*, lean_object*);
 LEAN_EXPORT lean_object* l_List_mapTR_loop___at___List_mapTR_loop___at___IVI_symmetriseLL_spec__1_spec__1(lean_object*, lean_object*, lean_object*);
 LEAN_EXPORT lean_object* l_IVI_Invariant_runUntilConverged(lean_object*, lean_object*, lean_object*, lean_object*);
-static lean_object* l_IVI_reprNonCollapseCfg___redArg___closed__3____x40_IVI_Invariant___hyg_1716_;
 uint8_t lean_nat_dec_eq(lean_object*, lean_object*);
 LEAN_EXPORT lean_object* l___private_IVI_Invariant_0__IVI_Invariant_lambdaVector_match__1_splitter(lean_object*, lean_object*, lean_object*, lean_object*, lean_object*, lean_object*, lean_object*);
 LEAN_EXPORT lean_object* l_IVI_surpriseNonDecreasing___boxed(lean_object*, lean_object*);
 static double l_IVI_surpriseNonDecreasing___closed__0;
 uint8_t lean_nat_dec_lt(lean_object*, lean_object*);
 lean_object* lean_nat_mod(lean_object*, lean_object*);
+static lean_object* l_IVI_reprNonCollapseCfg___redArg___closed__8____x40_IVI_Invariant___hyg_1654_;
 LEAN_EXPORT double l_IVI_Invariant_clampZero(double);
+LEAN_EXPORT lean_object* l_IVI_reprNonCollapseCfg____x40_IVI_Invariant___hyg_1654_(lean_object*, lean_object*);
 LEAN_EXPORT lean_object* l___private_IVI_Invariant_0__IVI_Invariant_lambdaVector_match__1_splitter___redArg(lean_object*, lean_object*, lean_object*, lean_object*, lean_object*, lean_object*);
 LEAN_EXPORT lean_object* l_IVI_Invariant_normalise(lean_object*);
-static lean_object* l_IVI_reprNonCollapseCfg___redArg___closed__1____x40_IVI_Invariant___hyg_1716_;
 LEAN_EXPORT lean_object* l_IVI_Invariant_powerIterAux___boxed(lean_object*, lean_object*, lean_object*, lean_object*, lean_object*);
 LEAN_EXPORT double l_IVI_Invariant_defaultWeighting___lam__0(lean_object*, lean_object*);
 LEAN_EXPORT lean_object* l_List_foldl___at___IVI_rowEntropy_spec__1___boxed(lean_object*, lean_object*, lean_object*);
@@ -134,33 +129,38 @@ LEAN_EXPORT double l_IVI_Invariant_defaultWeighting___lam__1(lean_object*, lean_
 lean_object* l_List_reverse___redArg(lean_object*);
 lean_object* lean_nat_sub(lean_object*, lean_object*);
 LEAN_EXPORT lean_object* l_IVI_Invariant_powerIterAux(lean_object*, double, lean_object*, double, lean_object*);
+static lean_object* l_IVI_reprNonCollapseCfg___redArg___closed__16____x40_IVI_Invariant___hyg_1654_;
 LEAN_EXPORT lean_object* l_List_mapTR_loop___at___IVI_symmetriseLL_spec__0___boxed__const__1;
 uint8_t lean_float_decLe(double, double);
 LEAN_EXPORT lean_object* l_IVI_symmetriseLL(lean_object*);
+static lean_object* l_IVI_reprNonCollapseCfg___redArg___closed__10____x40_IVI_Invariant___hyg_1654_;
+static lean_object* l_IVI_reprNonCollapseCfg___redArg___closed__14____x40_IVI_Invariant___hyg_1654_;
 LEAN_EXPORT double l_IVI_favg(double, double);
 LEAN_EXPORT lean_object* l_List_mapTR_loop___at___IVI_symmetriseLL_spec__0(lean_object*, lean_object*, lean_object*, lean_object*);
-static lean_object* l_IVI_reprNonCollapseCfg___redArg___closed__2____x40_IVI_Invariant___hyg_1716_;
 LEAN_EXPORT lean_object* l_List_mapTR_loop___at___IVI_symmetriseLL_spec__1(lean_object*, lean_object*, lean_object*);
 size_t lean_usize_sub(size_t, size_t);
 lean_object* lean_array_mk(lean_object*);
 LEAN_EXPORT double l_IVI_Invariant_spectralInvariantW(lean_object*, lean_object*);
 LEAN_EXPORT lean_object* l_IVI_Invariant_runUntilConverged_loop(lean_object*, lean_object*, lean_object*, lean_object*, lean_object*, lean_object*, double, lean_object*, lean_object*, lean_object*);
 LEAN_EXPORT lean_object* l_IVI_Invariant_defaultWeighting___lam__1___boxed(lean_object*, lean_object*);
+static lean_object* l_IVI_reprNonCollapseCfg___redArg___closed__13____x40_IVI_Invariant___hyg_1654_;
 lean_object* lean_array_uget(lean_object*, size_t);
 LEAN_EXPORT lean_object* l___private_IVI_Invariant_0__IVI_Invariant_powerIterAux_match__1_splitter___redArg(lean_object*, double, lean_object*, lean_object*, lean_object*);
 lean_object* l_List_zipWith___at___List_zip_spec__0___redArg(lean_object*, lean_object*);
+static lean_object* l_IVI_reprNonCollapseCfg___redArg___closed__2____x40_IVI_Invariant___hyg_1654_;
 LEAN_EXPORT lean_object* l_Array_foldrMUnsafe_fold___at___List_foldrTR___at___IVI_Invariant_coarse_spec__0_spec__0(lean_object*, size_t, size_t, lean_object*);
 double fabs(double);
 LEAN_EXPORT double l_List_foldl___at___IVI_Invariant_mulMatVec_spec__0(double, lean_object*);
 lean_object* lean_array_get_size(lean_object*);
 LEAN_EXPORT lean_object* l_List_mapTR_loop___at___IVI_Invariant_resonanceMatrixW_spec__2(double, lean_object*, lean_object*);
 LEAN_EXPORT lean_object* l_IVI_listGetD___boxed(lean_object*, lean_object*, lean_object*, lean_object*);
-static lean_object* l_IVI_reprNonCollapseCfg___redArg___closed__13____x40_IVI_Invariant___hyg_1716_;
 lean_object* lean_nat_add(lean_object*, lean_object*);
 LEAN_EXPORT lean_object* l_IVI_Invariant_enumerate___redArg(lean_object*);
 LEAN_EXPORT double l_IVI_Invariant_normInf(lean_object*);
 LEAN_EXPORT lean_object* l_IVI_Invariant_mulMatVec(lean_object*, lean_object*);
+static lean_object* l_IVI_reprNonCollapseCfg___redArg___closed__11____x40_IVI_Invariant___hyg_1654_;
 lean_object* l_List_drop___redArg(lean_object*, lean_object*);
+static lean_object* l_IVI_reprNonCollapseCfg___redArg___closed__12____x40_IVI_Invariant___hyg_1654_;
 LEAN_EXPORT lean_object* l_IVI_Invariant_resonanceMatrixW(lean_object*, lean_object*);
 LEAN_EXPORT lean_object* l_Array_foldrMUnsafe_fold___at___List_foldrTR___at___IVI_Invariant_coarse_spec__0_spec__0___boxed(lean_object*, lean_object*, lean_object*, lean_object*);
 double lean_float_sub(double, double);
@@ -2027,7 +2027,7 @@ lean_dec(x_1);
 return x_4;
 }
 }
-static lean_object* _init_l_IVI_reprNonCollapseCfg___redArg___closed__0____x40_IVI_Invariant___hyg_1716_() {
+static lean_object* _init_l_IVI_reprNonCollapseCfg___redArg___closed__0____x40_IVI_Invariant___hyg_1654_() {
 _start:
 {
 lean_object* x_1; 
@@ -2035,7 +2035,7 @@ x_1 = lean_mk_string_unchecked("{ ", 2, 2);
 return x_1;
 }
 }
-static lean_object* _init_l_IVI_reprNonCollapseCfg___redArg___closed__1____x40_IVI_Invariant___hyg_1716_() {
+static lean_object* _init_l_IVI_reprNonCollapseCfg___redArg___closed__1____x40_IVI_Invariant___hyg_1654_() {
 _start:
 {
 lean_object* x_1; 
@@ -2043,21 +2043,21 @@ x_1 = lean_mk_string_unchecked("epsLambda", 9, 9);
 return x_1;
 }
 }
-static lean_object* _init_l_IVI_reprNonCollapseCfg___redArg___closed__2____x40_IVI_Invariant___hyg_1716_() {
+static lean_object* _init_l_IVI_reprNonCollapseCfg___redArg___closed__2____x40_IVI_Invariant___hyg_1654_() {
 _start:
 {
 lean_object* x_1; lean_object* x_2; 
-x_1 = l_IVI_reprNonCollapseCfg___redArg___closed__1____x40_IVI_Invariant___hyg_1716_;
+x_1 = l_IVI_reprNonCollapseCfg___redArg___closed__1____x40_IVI_Invariant___hyg_1654_;
 x_2 = lean_alloc_ctor(3, 1, 0);
 lean_ctor_set(x_2, 0, x_1);
 return x_2;
 }
 }
-static lean_object* _init_l_IVI_reprNonCollapseCfg___redArg___closed__3____x40_IVI_Invariant___hyg_1716_() {
+static lean_object* _init_l_IVI_reprNonCollapseCfg___redArg___closed__3____x40_IVI_Invariant___hyg_1654_() {
 _start:
 {
 lean_object* x_1; lean_object* x_2; lean_object* x_3; 
-x_1 = l_IVI_reprNonCollapseCfg___redArg___closed__2____x40_IVI_Invariant___hyg_1716_;
+x_1 = l_IVI_reprNonCollapseCfg___redArg___closed__2____x40_IVI_Invariant___hyg_1654_;
 x_2 = lean_box(0);
 x_3 = lean_alloc_ctor(5, 2, 0);
 lean_ctor_set(x_3, 0, x_2);
@@ -2065,7 +2065,7 @@ lean_ctor_set(x_3, 1, x_1);
 return x_3;
 }
 }
-static lean_object* _init_l_IVI_reprNonCollapseCfg___redArg___closed__4____x40_IVI_Invariant___hyg_1716_() {
+static lean_object* _init_l_IVI_reprNonCollapseCfg___redArg___closed__4____x40_IVI_Invariant___hyg_1654_() {
 _start:
 {
 lean_object* x_1; 
@@ -2073,29 +2073,29 @@ x_1 = lean_mk_string_unchecked(" := ", 4, 4);
 return x_1;
 }
 }
-static lean_object* _init_l_IVI_reprNonCollapseCfg___redArg___closed__5____x40_IVI_Invariant___hyg_1716_() {
+static lean_object* _init_l_IVI_reprNonCollapseCfg___redArg___closed__5____x40_IVI_Invariant___hyg_1654_() {
 _start:
 {
 lean_object* x_1; lean_object* x_2; 
-x_1 = l_IVI_reprNonCollapseCfg___redArg___closed__4____x40_IVI_Invariant___hyg_1716_;
+x_1 = l_IVI_reprNonCollapseCfg___redArg___closed__4____x40_IVI_Invariant___hyg_1654_;
 x_2 = lean_alloc_ctor(3, 1, 0);
 lean_ctor_set(x_2, 0, x_1);
 return x_2;
 }
 }
-static lean_object* _init_l_IVI_reprNonCollapseCfg___redArg___closed__6____x40_IVI_Invariant___hyg_1716_() {
+static lean_object* _init_l_IVI_reprNonCollapseCfg___redArg___closed__6____x40_IVI_Invariant___hyg_1654_() {
 _start:
 {
 lean_object* x_1; lean_object* x_2; lean_object* x_3; 
-x_1 = l_IVI_reprNonCollapseCfg___redArg___closed__5____x40_IVI_Invariant___hyg_1716_;
-x_2 = l_IVI_reprNonCollapseCfg___redArg___closed__3____x40_IVI_Invariant___hyg_1716_;
+x_1 = l_IVI_reprNonCollapseCfg___redArg___closed__5____x40_IVI_Invariant___hyg_1654_;
+x_2 = l_IVI_reprNonCollapseCfg___redArg___closed__3____x40_IVI_Invariant___hyg_1654_;
 x_3 = lean_alloc_ctor(5, 2, 0);
 lean_ctor_set(x_3, 0, x_2);
 lean_ctor_set(x_3, 1, x_1);
 return x_3;
 }
 }
-static lean_object* _init_l_IVI_reprNonCollapseCfg___redArg___closed__7____x40_IVI_Invariant___hyg_1716_() {
+static lean_object* _init_l_IVI_reprNonCollapseCfg___redArg___closed__7____x40_IVI_Invariant___hyg_1654_() {
 _start:
 {
 lean_object* x_1; lean_object* x_2; 
@@ -2104,7 +2104,7 @@ x_2 = lean_nat_to_int(x_1);
 return x_2;
 }
 }
-static lean_object* _init_l_IVI_reprNonCollapseCfg___redArg___closed__8____x40_IVI_Invariant___hyg_1716_() {
+static lean_object* _init_l_IVI_reprNonCollapseCfg___redArg___closed__8____x40_IVI_Invariant___hyg_1654_() {
 _start:
 {
 lean_object* x_1; 
@@ -2112,17 +2112,17 @@ x_1 = lean_mk_string_unchecked(",", 1, 1);
 return x_1;
 }
 }
-static lean_object* _init_l_IVI_reprNonCollapseCfg___redArg___closed__9____x40_IVI_Invariant___hyg_1716_() {
+static lean_object* _init_l_IVI_reprNonCollapseCfg___redArg___closed__9____x40_IVI_Invariant___hyg_1654_() {
 _start:
 {
 lean_object* x_1; lean_object* x_2; 
-x_1 = l_IVI_reprNonCollapseCfg___redArg___closed__8____x40_IVI_Invariant___hyg_1716_;
+x_1 = l_IVI_reprNonCollapseCfg___redArg___closed__8____x40_IVI_Invariant___hyg_1654_;
 x_2 = lean_alloc_ctor(3, 1, 0);
 lean_ctor_set(x_2, 0, x_1);
 return x_2;
 }
 }
-static lean_object* _init_l_IVI_reprNonCollapseCfg___redArg___closed__10____x40_IVI_Invariant___hyg_1716_() {
+static lean_object* _init_l_IVI_reprNonCollapseCfg___redArg___closed__10____x40_IVI_Invariant___hyg_1654_() {
 _start:
 {
 lean_object* x_1; 
@@ -2130,17 +2130,17 @@ x_1 = lean_mk_string_unchecked("levels", 6, 6);
 return x_1;
 }
 }
-static lean_object* _init_l_IVI_reprNonCollapseCfg___redArg___closed__11____x40_IVI_Invariant___hyg_1716_() {
+static lean_object* _init_l_IVI_reprNonCollapseCfg___redArg___closed__11____x40_IVI_Invariant___hyg_1654_() {
 _start:
 {
 lean_object* x_1; lean_object* x_2; 
-x_1 = l_IVI_reprNonCollapseCfg___redArg___closed__10____x40_IVI_Invariant___hyg_1716_;
+x_1 = l_IVI_reprNonCollapseCfg___redArg___closed__10____x40_IVI_Invariant___hyg_1654_;
 x_2 = lean_alloc_ctor(3, 1, 0);
 lean_ctor_set(x_2, 0, x_1);
 return x_2;
 }
 }
-static lean_object* _init_l_IVI_reprNonCollapseCfg___redArg___closed__12____x40_IVI_Invariant___hyg_1716_() {
+static lean_object* _init_l_IVI_reprNonCollapseCfg___redArg___closed__12____x40_IVI_Invariant___hyg_1654_() {
 _start:
 {
 lean_object* x_1; lean_object* x_2; 
@@ -2149,7 +2149,7 @@ x_2 = lean_nat_to_int(x_1);
 return x_2;
 }
 }
-static lean_object* _init_l_IVI_reprNonCollapseCfg___redArg___closed__13____x40_IVI_Invariant___hyg_1716_() {
+static lean_object* _init_l_IVI_reprNonCollapseCfg___redArg___closed__13____x40_IVI_Invariant___hyg_1654_() {
 _start:
 {
 lean_object* x_1; 
@@ -2157,7 +2157,7 @@ x_1 = lean_mk_string_unchecked(" }", 2, 2);
 return x_1;
 }
 }
-static lean_object* _init_l_IVI_reprNonCollapseCfg___redArg___closed__14____x40_IVI_Invariant___hyg_1716_() {
+static lean_object* _init_l_IVI_reprNonCollapseCfg___redArg___closed__14____x40_IVI_Invariant___hyg_1654_() {
 _start:
 {
 lean_object* x_1; lean_object* x_2; 
@@ -2166,27 +2166,27 @@ x_2 = lean_nat_to_int(x_1);
 return x_2;
 }
 }
-static lean_object* _init_l_IVI_reprNonCollapseCfg___redArg___closed__15____x40_IVI_Invariant___hyg_1716_() {
+static lean_object* _init_l_IVI_reprNonCollapseCfg___redArg___closed__15____x40_IVI_Invariant___hyg_1654_() {
 _start:
 {
 lean_object* x_1; lean_object* x_2; 
-x_1 = l_IVI_reprNonCollapseCfg___redArg___closed__0____x40_IVI_Invariant___hyg_1716_;
+x_1 = l_IVI_reprNonCollapseCfg___redArg___closed__0____x40_IVI_Invariant___hyg_1654_;
 x_2 = lean_alloc_ctor(3, 1, 0);
 lean_ctor_set(x_2, 0, x_1);
 return x_2;
 }
 }
-static lean_object* _init_l_IVI_reprNonCollapseCfg___redArg___closed__16____x40_IVI_Invariant___hyg_1716_() {
+static lean_object* _init_l_IVI_reprNonCollapseCfg___redArg___closed__16____x40_IVI_Invariant___hyg_1654_() {
 _start:
 {
 lean_object* x_1; lean_object* x_2; 
-x_1 = l_IVI_reprNonCollapseCfg___redArg___closed__13____x40_IVI_Invariant___hyg_1716_;
+x_1 = l_IVI_reprNonCollapseCfg___redArg___closed__13____x40_IVI_Invariant___hyg_1654_;
 x_2 = lean_alloc_ctor(3, 1, 0);
 lean_ctor_set(x_2, 0, x_1);
 return x_2;
 }
 }
-LEAN_EXPORT lean_object* l_IVI_reprNonCollapseCfg___redArg____x40_IVI_Invariant___hyg_1716_(lean_object* x_1) {
+LEAN_EXPORT lean_object* l_IVI_reprNonCollapseCfg___redArg____x40_IVI_Invariant___hyg_1654_(lean_object* x_1) {
 _start:
 {
 double x_2; lean_object* x_3; lean_object* x_4; lean_object* x_5; lean_object* x_6; lean_object* x_7; lean_object* x_8; lean_object* x_9; lean_object* x_10; lean_object* x_11; uint8_t x_12; lean_object* x_13; lean_object* x_14; lean_object* x_15; lean_object* x_16; lean_object* x_17; lean_object* x_18; lean_object* x_19; lean_object* x_20; lean_object* x_21; lean_object* x_22; lean_object* x_23; lean_object* x_24; lean_object* x_25; uint8_t x_26; lean_object* x_27; lean_object* x_28; lean_object* x_29; lean_object* x_30; lean_object* x_31; lean_object* x_32; lean_object* x_33; lean_object* x_34; uint8_t x_35; 
@@ -2194,9 +2194,9 @@ x_2 = lean_ctor_get_float(x_1, sizeof(void*)*1);
 x_3 = lean_ctor_get(x_1, 0);
 lean_inc(x_3);
 lean_dec(x_1);
-x_4 = l_IVI_reprNonCollapseCfg___redArg___closed__5____x40_IVI_Invariant___hyg_1716_;
-x_5 = l_IVI_reprNonCollapseCfg___redArg___closed__6____x40_IVI_Invariant___hyg_1716_;
-x_6 = l_IVI_reprNonCollapseCfg___redArg___closed__7____x40_IVI_Invariant___hyg_1716_;
+x_4 = l_IVI_reprNonCollapseCfg___redArg___closed__5____x40_IVI_Invariant___hyg_1654_;
+x_5 = l_IVI_reprNonCollapseCfg___redArg___closed__6____x40_IVI_Invariant___hyg_1654_;
+x_6 = l_IVI_reprNonCollapseCfg___redArg___closed__7____x40_IVI_Invariant___hyg_1654_;
 x_7 = lean_unsigned_to_nat(0u);
 x_8 = l_Float_repr(x_2, x_7);
 x_9 = lean_alloc_ctor(4, 2, 0);
@@ -2210,7 +2210,7 @@ lean_ctor_set_uint8(x_11, sizeof(void*)*1, x_12);
 x_13 = lean_alloc_ctor(5, 2, 0);
 lean_ctor_set(x_13, 0, x_5);
 lean_ctor_set(x_13, 1, x_11);
-x_14 = l_IVI_reprNonCollapseCfg___redArg___closed__9____x40_IVI_Invariant___hyg_1716_;
+x_14 = l_IVI_reprNonCollapseCfg___redArg___closed__9____x40_IVI_Invariant___hyg_1654_;
 x_15 = lean_alloc_ctor(5, 2, 0);
 lean_ctor_set(x_15, 0, x_13);
 lean_ctor_set(x_15, 1, x_14);
@@ -2218,14 +2218,14 @@ x_16 = lean_box(1);
 x_17 = lean_alloc_ctor(5, 2, 0);
 lean_ctor_set(x_17, 0, x_15);
 lean_ctor_set(x_17, 1, x_16);
-x_18 = l_IVI_reprNonCollapseCfg___redArg___closed__11____x40_IVI_Invariant___hyg_1716_;
+x_18 = l_IVI_reprNonCollapseCfg___redArg___closed__11____x40_IVI_Invariant___hyg_1654_;
 x_19 = lean_alloc_ctor(5, 2, 0);
 lean_ctor_set(x_19, 0, x_17);
 lean_ctor_set(x_19, 1, x_18);
 x_20 = lean_alloc_ctor(5, 2, 0);
 lean_ctor_set(x_20, 0, x_19);
 lean_ctor_set(x_20, 1, x_4);
-x_21 = l_IVI_reprNonCollapseCfg___redArg___closed__12____x40_IVI_Invariant___hyg_1716_;
+x_21 = l_IVI_reprNonCollapseCfg___redArg___closed__12____x40_IVI_Invariant___hyg_1654_;
 x_22 = l_Nat_reprFast(x_3);
 x_23 = lean_alloc_ctor(3, 1, 0);
 lean_ctor_set(x_23, 0, x_22);
@@ -2239,12 +2239,12 @@ lean_ctor_set_uint8(x_25, sizeof(void*)*1, x_26);
 x_27 = lean_alloc_ctor(5, 2, 0);
 lean_ctor_set(x_27, 0, x_20);
 lean_ctor_set(x_27, 1, x_25);
-x_28 = l_IVI_reprNonCollapseCfg___redArg___closed__14____x40_IVI_Invariant___hyg_1716_;
-x_29 = l_IVI_reprNonCollapseCfg___redArg___closed__15____x40_IVI_Invariant___hyg_1716_;
+x_28 = l_IVI_reprNonCollapseCfg___redArg___closed__14____x40_IVI_Invariant___hyg_1654_;
+x_29 = l_IVI_reprNonCollapseCfg___redArg___closed__15____x40_IVI_Invariant___hyg_1654_;
 x_30 = lean_alloc_ctor(5, 2, 0);
 lean_ctor_set(x_30, 0, x_29);
 lean_ctor_set(x_30, 1, x_27);
-x_31 = l_IVI_reprNonCollapseCfg___redArg___closed__16____x40_IVI_Invariant___hyg_1716_;
+x_31 = l_IVI_reprNonCollapseCfg___redArg___closed__16____x40_IVI_Invariant___hyg_1654_;
 x_32 = lean_alloc_ctor(5, 2, 0);
 lean_ctor_set(x_32, 0, x_30);
 lean_ctor_set(x_32, 1, x_31);
@@ -2258,19 +2258,19 @@ lean_ctor_set_uint8(x_34, sizeof(void*)*1, x_35);
 return x_34;
 }
 }
-LEAN_EXPORT lean_object* l_IVI_reprNonCollapseCfg____x40_IVI_Invariant___hyg_1716_(lean_object* x_1, lean_object* x_2) {
+LEAN_EXPORT lean_object* l_IVI_reprNonCollapseCfg____x40_IVI_Invariant___hyg_1654_(lean_object* x_1, lean_object* x_2) {
 _start:
 {
 lean_object* x_3; 
-x_3 = l_IVI_reprNonCollapseCfg___redArg____x40_IVI_Invariant___hyg_1716_(x_1);
+x_3 = l_IVI_reprNonCollapseCfg___redArg____x40_IVI_Invariant___hyg_1654_(x_1);
 return x_3;
 }
 }
-LEAN_EXPORT lean_object* l_IVI_reprNonCollapseCfg____x40_IVI_Invariant___hyg_1716____boxed(lean_object* x_1, lean_object* x_2) {
+LEAN_EXPORT lean_object* l_IVI_reprNonCollapseCfg____x40_IVI_Invariant___hyg_1654____boxed(lean_object* x_1, lean_object* x_2) {
 _start:
 {
 lean_object* x_3; 
-x_3 = l_IVI_reprNonCollapseCfg____x40_IVI_Invariant___hyg_1716_(x_1, x_2);
+x_3 = l_IVI_reprNonCollapseCfg____x40_IVI_Invariant___hyg_1654_(x_1, x_2);
 lean_dec(x_2);
 return x_3;
 }
@@ -2279,7 +2279,7 @@ static lean_object* _init_l_IVI_instReprNonCollapseCfg___closed__0() {
 _start:
 {
 lean_object* x_1; 
-x_1 = lean_alloc_closure((void*)(l_IVI_reprNonCollapseCfg____x40_IVI_Invariant___hyg_1716____boxed), 2, 0);
+x_1 = lean_alloc_closure((void*)(l_IVI_reprNonCollapseCfg____x40_IVI_Invariant___hyg_1654____boxed), 2, 0);
 return x_1;
 }
 }
@@ -2581,40 +2581,40 @@ l_IVI_Invariant_spectralInvariantW___closed__0 = _init_l_IVI_Invariant_spectralI
 l_IVI_favg___closed__0 = _init_l_IVI_favg___closed__0();
 l_List_mapTR_loop___at___IVI_symmetriseLL_spec__0___boxed__const__1 = _init_l_List_mapTR_loop___at___IVI_symmetriseLL_spec__0___boxed__const__1();
 lean_mark_persistent(l_List_mapTR_loop___at___IVI_symmetriseLL_spec__0___boxed__const__1);
-l_IVI_reprNonCollapseCfg___redArg___closed__0____x40_IVI_Invariant___hyg_1716_ = _init_l_IVI_reprNonCollapseCfg___redArg___closed__0____x40_IVI_Invariant___hyg_1716_();
-lean_mark_persistent(l_IVI_reprNonCollapseCfg___redArg___closed__0____x40_IVI_Invariant___hyg_1716_);
-l_IVI_reprNonCollapseCfg___redArg___closed__1____x40_IVI_Invariant___hyg_1716_ = _init_l_IVI_reprNonCollapseCfg___redArg___closed__1____x40_IVI_Invariant___hyg_1716_();
-lean_mark_persistent(l_IVI_reprNonCollapseCfg___redArg___closed__1____x40_IVI_Invariant___hyg_1716_);
-l_IVI_reprNonCollapseCfg___redArg___closed__2____x40_IVI_Invariant___hyg_1716_ = _init_l_IVI_reprNonCollapseCfg___redArg___closed__2____x40_IVI_Invariant___hyg_1716_();
-lean_mark_persistent(l_IVI_reprNonCollapseCfg___redArg___closed__2____x40_IVI_Invariant___hyg_1716_);
-l_IVI_reprNonCollapseCfg___redArg___closed__3____x40_IVI_Invariant___hyg_1716_ = _init_l_IVI_reprNonCollapseCfg___redArg___closed__3____x40_IVI_Invariant___hyg_1716_();
-lean_mark_persistent(l_IVI_reprNonCollapseCfg___redArg___closed__3____x40_IVI_Invariant___hyg_1716_);
-l_IVI_reprNonCollapseCfg___redArg___closed__4____x40_IVI_Invariant___hyg_1716_ = _init_l_IVI_reprNonCollapseCfg___redArg___closed__4____x40_IVI_Invariant___hyg_1716_();
-lean_mark_persistent(l_IVI_reprNonCollapseCfg___redArg___closed__4____x40_IVI_Invariant___hyg_1716_);
-l_IVI_reprNonCollapseCfg___redArg___closed__5____x40_IVI_Invariant___hyg_1716_ = _init_l_IVI_reprNonCollapseCfg___redArg___closed__5____x40_IVI_Invariant___hyg_1716_();
-lean_mark_persistent(l_IVI_reprNonCollapseCfg___redArg___closed__5____x40_IVI_Invariant___hyg_1716_);
-l_IVI_reprNonCollapseCfg___redArg___closed__6____x40_IVI_Invariant___hyg_1716_ = _init_l_IVI_reprNonCollapseCfg___redArg___closed__6____x40_IVI_Invariant___hyg_1716_();
-lean_mark_persistent(l_IVI_reprNonCollapseCfg___redArg___closed__6____x40_IVI_Invariant___hyg_1716_);
-l_IVI_reprNonCollapseCfg___redArg___closed__7____x40_IVI_Invariant___hyg_1716_ = _init_l_IVI_reprNonCollapseCfg___redArg___closed__7____x40_IVI_Invariant___hyg_1716_();
-lean_mark_persistent(l_IVI_reprNonCollapseCfg___redArg___closed__7____x40_IVI_Invariant___hyg_1716_);
-l_IVI_reprNonCollapseCfg___redArg___closed__8____x40_IVI_Invariant___hyg_1716_ = _init_l_IVI_reprNonCollapseCfg___redArg___closed__8____x40_IVI_Invariant___hyg_1716_();
-lean_mark_persistent(l_IVI_reprNonCollapseCfg___redArg___closed__8____x40_IVI_Invariant___hyg_1716_);
-l_IVI_reprNonCollapseCfg___redArg___closed__9____x40_IVI_Invariant___hyg_1716_ = _init_l_IVI_reprNonCollapseCfg___redArg___closed__9____x40_IVI_Invariant___hyg_1716_();
-lean_mark_persistent(l_IVI_reprNonCollapseCfg___redArg___closed__9____x40_IVI_Invariant___hyg_1716_);
-l_IVI_reprNonCollapseCfg___redArg___closed__10____x40_IVI_Invariant___hyg_1716_ = _init_l_IVI_reprNonCollapseCfg___redArg___closed__10____x40_IVI_Invariant___hyg_1716_();
-lean_mark_persistent(l_IVI_reprNonCollapseCfg___redArg___closed__10____x40_IVI_Invariant___hyg_1716_);
-l_IVI_reprNonCollapseCfg___redArg___closed__11____x40_IVI_Invariant___hyg_1716_ = _init_l_IVI_reprNonCollapseCfg___redArg___closed__11____x40_IVI_Invariant___hyg_1716_();
-lean_mark_persistent(l_IVI_reprNonCollapseCfg___redArg___closed__11____x40_IVI_Invariant___hyg_1716_);
-l_IVI_reprNonCollapseCfg___redArg___closed__12____x40_IVI_Invariant___hyg_1716_ = _init_l_IVI_reprNonCollapseCfg___redArg___closed__12____x40_IVI_Invariant___hyg_1716_();
-lean_mark_persistent(l_IVI_reprNonCollapseCfg___redArg___closed__12____x40_IVI_Invariant___hyg_1716_);
-l_IVI_reprNonCollapseCfg___redArg___closed__13____x40_IVI_Invariant___hyg_1716_ = _init_l_IVI_reprNonCollapseCfg___redArg___closed__13____x40_IVI_Invariant___hyg_1716_();
-lean_mark_persistent(l_IVI_reprNonCollapseCfg___redArg___closed__13____x40_IVI_Invariant___hyg_1716_);
-l_IVI_reprNonCollapseCfg___redArg___closed__14____x40_IVI_Invariant___hyg_1716_ = _init_l_IVI_reprNonCollapseCfg___redArg___closed__14____x40_IVI_Invariant___hyg_1716_();
-lean_mark_persistent(l_IVI_reprNonCollapseCfg___redArg___closed__14____x40_IVI_Invariant___hyg_1716_);
-l_IVI_reprNonCollapseCfg___redArg___closed__15____x40_IVI_Invariant___hyg_1716_ = _init_l_IVI_reprNonCollapseCfg___redArg___closed__15____x40_IVI_Invariant___hyg_1716_();
-lean_mark_persistent(l_IVI_reprNonCollapseCfg___redArg___closed__15____x40_IVI_Invariant___hyg_1716_);
-l_IVI_reprNonCollapseCfg___redArg___closed__16____x40_IVI_Invariant___hyg_1716_ = _init_l_IVI_reprNonCollapseCfg___redArg___closed__16____x40_IVI_Invariant___hyg_1716_();
-lean_mark_persistent(l_IVI_reprNonCollapseCfg___redArg___closed__16____x40_IVI_Invariant___hyg_1716_);
+l_IVI_reprNonCollapseCfg___redArg___closed__0____x40_IVI_Invariant___hyg_1654_ = _init_l_IVI_reprNonCollapseCfg___redArg___closed__0____x40_IVI_Invariant___hyg_1654_();
+lean_mark_persistent(l_IVI_reprNonCollapseCfg___redArg___closed__0____x40_IVI_Invariant___hyg_1654_);
+l_IVI_reprNonCollapseCfg___redArg___closed__1____x40_IVI_Invariant___hyg_1654_ = _init_l_IVI_reprNonCollapseCfg___redArg___closed__1____x40_IVI_Invariant___hyg_1654_();
+lean_mark_persistent(l_IVI_reprNonCollapseCfg___redArg___closed__1____x40_IVI_Invariant___hyg_1654_);
+l_IVI_reprNonCollapseCfg___redArg___closed__2____x40_IVI_Invariant___hyg_1654_ = _init_l_IVI_reprNonCollapseCfg___redArg___closed__2____x40_IVI_Invariant___hyg_1654_();
+lean_mark_persistent(l_IVI_reprNonCollapseCfg___redArg___closed__2____x40_IVI_Invariant___hyg_1654_);
+l_IVI_reprNonCollapseCfg___redArg___closed__3____x40_IVI_Invariant___hyg_1654_ = _init_l_IVI_reprNonCollapseCfg___redArg___closed__3____x40_IVI_Invariant___hyg_1654_();
+lean_mark_persistent(l_IVI_reprNonCollapseCfg___redArg___closed__3____x40_IVI_Invariant___hyg_1654_);
+l_IVI_reprNonCollapseCfg___redArg___closed__4____x40_IVI_Invariant___hyg_1654_ = _init_l_IVI_reprNonCollapseCfg___redArg___closed__4____x40_IVI_Invariant___hyg_1654_();
+lean_mark_persistent(l_IVI_reprNonCollapseCfg___redArg___closed__4____x40_IVI_Invariant___hyg_1654_);
+l_IVI_reprNonCollapseCfg___redArg___closed__5____x40_IVI_Invariant___hyg_1654_ = _init_l_IVI_reprNonCollapseCfg___redArg___closed__5____x40_IVI_Invariant___hyg_1654_();
+lean_mark_persistent(l_IVI_reprNonCollapseCfg___redArg___closed__5____x40_IVI_Invariant___hyg_1654_);
+l_IVI_reprNonCollapseCfg___redArg___closed__6____x40_IVI_Invariant___hyg_1654_ = _init_l_IVI_reprNonCollapseCfg___redArg___closed__6____x40_IVI_Invariant___hyg_1654_();
+lean_mark_persistent(l_IVI_reprNonCollapseCfg___redArg___closed__6____x40_IVI_Invariant___hyg_1654_);
+l_IVI_reprNonCollapseCfg___redArg___closed__7____x40_IVI_Invariant___hyg_1654_ = _init_l_IVI_reprNonCollapseCfg___redArg___closed__7____x40_IVI_Invariant___hyg_1654_();
+lean_mark_persistent(l_IVI_reprNonCollapseCfg___redArg___closed__7____x40_IVI_Invariant___hyg_1654_);
+l_IVI_reprNonCollapseCfg___redArg___closed__8____x40_IVI_Invariant___hyg_1654_ = _init_l_IVI_reprNonCollapseCfg___redArg___closed__8____x40_IVI_Invariant___hyg_1654_();
+lean_mark_persistent(l_IVI_reprNonCollapseCfg___redArg___closed__8____x40_IVI_Invariant___hyg_1654_);
+l_IVI_reprNonCollapseCfg___redArg___closed__9____x40_IVI_Invariant___hyg_1654_ = _init_l_IVI_reprNonCollapseCfg___redArg___closed__9____x40_IVI_Invariant___hyg_1654_();
+lean_mark_persistent(l_IVI_reprNonCollapseCfg___redArg___closed__9____x40_IVI_Invariant___hyg_1654_);
+l_IVI_reprNonCollapseCfg___redArg___closed__10____x40_IVI_Invariant___hyg_1654_ = _init_l_IVI_reprNonCollapseCfg___redArg___closed__10____x40_IVI_Invariant___hyg_1654_();
+lean_mark_persistent(l_IVI_reprNonCollapseCfg___redArg___closed__10____x40_IVI_Invariant___hyg_1654_);
+l_IVI_reprNonCollapseCfg___redArg___closed__11____x40_IVI_Invariant___hyg_1654_ = _init_l_IVI_reprNonCollapseCfg___redArg___closed__11____x40_IVI_Invariant___hyg_1654_();
+lean_mark_persistent(l_IVI_reprNonCollapseCfg___redArg___closed__11____x40_IVI_Invariant___hyg_1654_);
+l_IVI_reprNonCollapseCfg___redArg___closed__12____x40_IVI_Invariant___hyg_1654_ = _init_l_IVI_reprNonCollapseCfg___redArg___closed__12____x40_IVI_Invariant___hyg_1654_();
+lean_mark_persistent(l_IVI_reprNonCollapseCfg___redArg___closed__12____x40_IVI_Invariant___hyg_1654_);
+l_IVI_reprNonCollapseCfg___redArg___closed__13____x40_IVI_Invariant___hyg_1654_ = _init_l_IVI_reprNonCollapseCfg___redArg___closed__13____x40_IVI_Invariant___hyg_1654_();
+lean_mark_persistent(l_IVI_reprNonCollapseCfg___redArg___closed__13____x40_IVI_Invariant___hyg_1654_);
+l_IVI_reprNonCollapseCfg___redArg___closed__14____x40_IVI_Invariant___hyg_1654_ = _init_l_IVI_reprNonCollapseCfg___redArg___closed__14____x40_IVI_Invariant___hyg_1654_();
+lean_mark_persistent(l_IVI_reprNonCollapseCfg___redArg___closed__14____x40_IVI_Invariant___hyg_1654_);
+l_IVI_reprNonCollapseCfg___redArg___closed__15____x40_IVI_Invariant___hyg_1654_ = _init_l_IVI_reprNonCollapseCfg___redArg___closed__15____x40_IVI_Invariant___hyg_1654_();
+lean_mark_persistent(l_IVI_reprNonCollapseCfg___redArg___closed__15____x40_IVI_Invariant___hyg_1654_);
+l_IVI_reprNonCollapseCfg___redArg___closed__16____x40_IVI_Invariant___hyg_1654_ = _init_l_IVI_reprNonCollapseCfg___redArg___closed__16____x40_IVI_Invariant___hyg_1654_();
+lean_mark_persistent(l_IVI_reprNonCollapseCfg___redArg___closed__16____x40_IVI_Invariant___hyg_1654_);
 l_IVI_instReprNonCollapseCfg___closed__0 = _init_l_IVI_instReprNonCollapseCfg___closed__0();
 lean_mark_persistent(l_IVI_instReprNonCollapseCfg___closed__0);
 l_IVI_instReprNonCollapseCfg = _init_l_IVI_instReprNonCollapseCfg();
